specs/Spec.Blake2_Vec.fst
@@ -1,0 +1,508 @@
+module Spec.Blake2_Vec
+
+open FStar.Mul
+open Lib.IntTypes
+open Lib.RawIntTypes
+open Lib.Sequence
+open Lib.ByteSequence
+open Lib.LoopCombinators
+
+#set-options "--z3rlimit 50"
+
+type alg =
+  | Blake2S
+  | Blake2B
+
+inline_for_extraction
+let wt (a:alg) : t:inttype{unsigned t} =
+  match a with
+  | Blake2S -> U32
+  | Blake2B -> U64
+
+inline_for_extraction
+let rounds (a:alg) =
+  match a with
+  | Blake2S -> 10
+  | Blake2B -> 12
+
+(* Algorithm parameters *)
+inline_for_extraction let size_hash_w : size_nat = 8
+inline_for_extraction let size_block_w : size_nat = 16
+inline_for_extraction let size_word (a:alg) : size_nat = numbytes (wt a)
+inline_for_extraction let size_block (a:alg) : size_nat = size_block_w * (size_word a)
+inline_for_extraction let size_ivTable : size_nat = 8
+inline_for_extraction let size_sigmaTable : size_nat = 160
+
+inline_for_extraction let max_key (a:alg) =
+  match a with
+  | Blake2S -> 32
+  | Blake2B -> 64
+inline_for_extraction let max_output (a:alg) =
+  match a with
+  | Blake2S -> 32
+  | Blake2B -> 64
+
+
+(* Definition of base types *)
+inline_for_extraction
+unfold let limb_inttype (a:alg) =
+  match (wt a) with
+  | U32 -> U64
+  | U64 -> U128
+
+inline_for_extraction
+unfold type word_t (a:alg) = uint_t (wt a) SEC
+
+inline_for_extraction
+let zero (a:alg) : word_t a=
+  match a with
+  | Blake2S -> u32 0
+  | Blake2B -> u64 0
+
+inline_for_extraction
+unfold let row (a:alg) = lseq (word_t a) 4
+
+inline_for_extraction
+let zero_row (a:alg) : row a = create 4 (zero a)
+
+inline_for_extraction
+let load_row (#a:alg) (s:lseq (word_t a) 4) : row a =
+  createL [s.[0]; s.[1]; s.[2]; s.[3]]
+
+inline_for_extraction
+let create_row (#a:alg) x0 x1 x2 x3 : row a =
+  createL [x0;x1;x2;x3]
+
+inline_for_extraction
+unfold let row2 (a:alg) = lseq (row a) 2
+
+inline_for_extraction
+unfold let vector (a:alg) = lseq (row a) 4
+
+inline_for_extraction
+let zero_vector (a:alg) : vector a = create 4 (zero_row a)
+
+
+inline_for_extraction
+type pub_word_t (a:alg) = uint_t (wt a) PUB
+
+inline_for_extraction
+type limb_t (a:alg) : Type0 = uint_t (limb_inttype a) SEC
+
+inline_for_extraction
+let max_limb (a:alg) = maxint (limb_inttype a)
+
+inline_for_extraction
+let nat_to_word (a:alg) (x:size_nat) : word_t a =
+  match (wt a) with
+  | U32 -> u32 x
+  | U64 -> u64 x
+
+inline_for_extraction
+let nat_to_limb (a:alg) (x:nat{x <= max_limb a}) : xl:limb_t a{uint_v xl == x} =
+  match (wt a) with
+  | U32 -> u64 x
+  | U64 -> admit(); u128 x
+
+inline_for_extraction
+let word_to_limb (a:alg) (x:word_t a{uint_v x <= max_limb a}) : xl:limb_t a{uint_v xl == uint_v x} =
+  match (wt a) with
+  | U32 -> to_u64 x
+  | U64 -> to_u128 x
+
+inline_for_extraction
+let limb_to_word (a:alg) (x:limb_t a) : word_t a =
+  match (wt a) with
+  | U32 -> to_u32 x
+  | U64 -> to_u64 x
+
+unfold let rtable_t (a:alg) = lseq (rotval (wt a)) 4
+
+[@"opaque_to_smt"]
+inline_for_extraction
+let rTable_list_S : l:List.Tot.llist (rotval U32) 4 =
+  [
+    size 16; size 12; size 8; size 7
+  ]
+
+[@"opaque_to_smt"]
+inline_for_extraction
+let rTable_list_B: l:List.Tot.llist (rotval U64) 4 =
+  [
+    size 32; size 24; size 16; size 63
+  ]
+
+inline_for_extraction
+let rTable (a:alg) : rtable_t a =
+  match a with
+  | Blake2S -> (of_list rTable_list_S)
+  | Blake2B -> (of_list rTable_list_B)
+
+[@"opaque_to_smt"]
+inline_for_extraction
+let list_iv_S: l:List.Tot.llist (uint_t U32 PUB) 8 =
+  [@inline_let]
+  let l = [
+    0x6A09E667ul; 0xBB67AE85ul; 0x3C6EF372ul; 0xA54FF53Aul;
+    0x510E527Ful; 0x9B05688Cul; 0x1F83D9ABul; 0x5BE0CD19ul] in
+  assert_norm(List.Tot.length l == 8);
+  l
+
+[@"opaque_to_smt"]
+inline_for_extraction
+let list_iv_B: List.Tot.llist (uint_t U64 PUB) 8 =
+  [@inline_let]
+  let l = [
+    0x6A09E667F3BCC908uL; 0xBB67AE8584CAA73BuL;
+    0x3C6EF372FE94F82BuL; 0xA54FF53A5F1D36F1uL;
+    0x510E527FADE682D1uL; 0x9B05688C2B3E6C1FuL;
+    0x1F83D9ABFB41BD6BuL; 0x5BE0CD19137E2179uL] in
+  assert_norm(List.Tot.length l == 8);
+  l
+
+[@"opaque_to_smt"]
+inline_for_extraction
+let list_iv (a:alg): List.Tot.llist (pub_word_t a) 8 =
+  match a with
+  | Blake2S -> list_iv_S
+  | Blake2B -> list_iv_B
+
+inline_for_extraction
+let ivTable (a:alg) : lseq (pub_word_t a) 8 =
+  match a with
+  | Blake2S -> of_list list_iv_S
+  | Blake2B -> of_list list_iv_B
+
+type sigma_elt_t = n:size_t{size_v n < 16}
+type list_sigma_t = l:list sigma_elt_t{List.Tot.length l == 160}
+
+let list_sigma: list_sigma_t =
+  [@inline_let]
+  let l : list sigma_elt_t = [
+    size  0; size  1; size  2; size  3; size  4; size  5; size  6; size  7;
+    size  8; size  9; size 10; size 11; size 12; size 13; size 14; size 15;
+    size 14; size 10; size  4; size  8; size  9; size 15; size 13; size  6;
+    size  1; size 12; size  0; size  2; size 11; size  7; size  5; size  3;
+    size 11; size  8; size 12; size  0; size  5; size  2; size 15; size 13;
+    size 10; size 14; size  3; size  6; size  7; size  1; size  9; size  4;
+    size  7; size  9; size  3; size  1; size 13; size 12; size 11; size 14;
+    size  2; size  6; size  5; size 10; size  4; size  0; size 15; size  8;
+    size  9; size  0; size  5; size  7; size  2; size  4; size 10; size 15;
+    size 14; size  1; size 11; size 12; size  6; size  8; size  3; size 13;
+    size  2; size 12; size  6; size 10; size  0; size 11; size  8; size  3;
+    size  4; size 13; size  7; size  5; size 15; size 14; size  1; size  9;
+    size 12; size  5; size  1; size 15; size 14; size 13; size  4; size 10;
+    size  0; size  7; size  6; size  3; size  9; size  2; size  8; size 11;
+    size 13; size 11; size  7; size 14; size 12; size  1; size  3; size  9;
+    size  5; size  0; size 15; size  4; size  8; size  6; size  2; size 10;
+    size  6; size 15; size 14; size  9; size 11; size  3; size  0; size  8;
+    size 12; size  2; size 13; size  7; size  1; size  4; size 10; size  5;
+    size 10; size  2; size  8; size  4; size  7; size  6; size  1; size  5;
+    size 15; size 11; size  9; size 14; size  3; size 12; size 13; size  0
+    ] in
+  assert_norm(List.Tot.length l == 160);
+  l
+
+
+inline_for_extraction
+let sigmaTable:lseq sigma_elt_t size_sigmaTable =
+  assert_norm (List.Tot.length list_sigma == size_sigmaTable);
+  of_list list_sigma
+
+
+(* Algorithms types *)
+type vector_ws (a:alg) = lseq (word_t a) size_block_w
+type block_ws (a:alg) = lseq (word_t a) size_block_w
+type block_s (a:alg) = lseq uint8 (size_block a)
+type hash_ws (a:alg) = lseq (word_t a) size_hash_w
+type idx_t = n:size_nat{n < 16}
+
+let row_idx = n:nat {n < 4}
+
+inline_for_extraction
+let gather_row (#a:alg) (m:block_s a) (i0 i1 i2 i3:sigma_elt_t) : row a =
+  let nb = size_word a in
+  let u0 = uint_from_bytes_le #(wt a) #SEC (sub m (v i0*nb) nb) in
+  let u1 = uint_from_bytes_le #(wt a) #SEC (sub m (v i1*nb) nb) in
+  let u2 = uint_from_bytes_le #(wt a) #SEC (sub m (v i2*nb) nb) in
+  let u3 = uint_from_bytes_le #(wt a) #SEC (sub m (v i3*nb) nb) in
+  create_row u0 u1 u2 u3
+
+
+inline_for_extraction
+let ( ^| ) (#a:alg) (r1:row a) (r2:row a) : row a =
+  map2 ( ^. ) r1 r2
+
+inline_for_extraction
+let ( +| ) (#a:alg) (r1:row a) (r2:row a) : row a =
+  map2 ( +. ) r1 r2
+
+inline_for_extraction
+let ( >>>| ) (#a:alg) (r1:row a) (r:rotval (wt a)) : row a =
+  map #(word_t a) ( fun x -> x >>>. r) r1
+
+inline_for_extraction
+let rotr (#a:alg) (r1:row a) (r:row_idx) : row a =
+  createi 4 (fun i -> r1.[(i+r)%4])
+
+
+(* Functions *)
+let g1 (a:alg) (wv:vector a) (i:row_idx) (j:row_idx) (r:rotval (wt a)) : Tot (vector a) =
+  wv.[i] <- (wv.[i] ^| wv.[j]) >>>| r
+
+let g2 (a:alg) (wv:vector a) (i:row_idx) (j:row_idx) (x:row a) : Tot (vector a) =
+  wv.[i] <- (wv.[i] +| wv.[j] +| x)
+
+
+val blake2_mixing:
+    a:alg
+  -> ws:vector a
+  -> row_idx
+  -> row_idx
+  -> row_idx
+  -> row_idx
+  -> row a
+  -> row a ->
+  Tot (vector a)
+
+let blake2_mixing al wv a b c d x y =
+  let rt = rTable al in
+  let wv = g2 al wv a b x in
+  let wv = g1 al wv d a rt.[0] in
+  let wv = g2 al wv c d (zero_row al) in
+  let wv = g1 al wv b c rt.[1] in
+  let wv = g2 al wv a b y in
+  let wv = g1 al wv d a rt.[2] in
+  let wv = g2 al wv c d (zero_row al) in
+  let wv = g1 al wv b c rt.[3] in
+  wv
+
+let diag (#a:alg) (wv:vector a) : vector a =
+  let wv = wv.[1] <- rotr wv.[1] 1 in
+  let wv = wv.[2] <- rotr wv.[2] 2 in
+  let wv = wv.[3] <- rotr wv.[3] 3 in
+  wv
+
+let undiag (#a:alg) (wv:vector a) : vector a =
+  let wv = wv.[1] <- rotr wv.[1] 3 in
+  let wv = wv.[2] <- rotr wv.[2] 2 in
+  let wv = wv.[3] <- rotr wv.[3] 1 in
+  wv
+
+val blake2_round:
+    a:alg
+  -> m:block_s a
+  -> i:size_nat
+  -> wv:vector a
+  -> vector a
+
+let blake2_round a m i wv =
+  let start = (i%10) * 16 in
+  let x = gather_row m sigmaTable.[start] sigmaTable.[start+2] sigmaTable.[start+4] sigmaTable.[start+6]  in
+  let y = gather_row m sigmaTable.[start+1] sigmaTable.[start+3] sigmaTable.[start+5] sigmaTable.[start+7]  in
+  let z = gather_row m sigmaTable.[start+8] sigmaTable.[start+10] sigmaTable.[start+12] sigmaTable.[start+14]  in
+  let w = gather_row m sigmaTable.[start+9] sigmaTable.[start+11] sigmaTable.[start+13] sigmaTable.[start+15]  in
+  let wv = blake2_mixing a wv 0 1 2 3 x y in
+  let wv = diag wv in
+  let wv = blake2_mixing a wv 0 1 2 3 z w in
+  undiag wv
+
+
+val blake2_compress1:
+    a:alg
+  -> iv:row2 a
+  -> s:row2 a
+  -> offset:limb_t a
+  -> flag:bool ->
+  Tot (vector a)
+
+let blake2_compress1 a iv s offset flag =
+  let wv : vector a = s @| iv in
+  let low_offset = limb_to_word a offset in
+  let high_offset = limb_to_word a (shift_right #(limb_inttype a) offset (size (bits (wt a)))) in
+  let m_12 = low_offset in
+  let m_13 = high_offset in
+  let m_14 = if flag then (ones (wt a) SEC) else zero a in
+  let m_15 = zero a in
+  let mask = create_row m_12 m_13 m_14 m_15 in
+  let wv = wv.[3] <- wv.[3] ^| mask in
+  wv
+
+
+val blake2_compress2:
+    a:alg
+  -> wv:vector a
+  -> m:block_s a ->
+  Tot (vector a)
+
+let blake2_compress2 a wv m = repeati (rounds a) (blake2_round a m) wv
+
+val blake2_compress3:
+    a:alg
+  -> wv:vector a
+  -> s:row2 a ->
+  Tot (row2 a)
+
+let blake2_compress3 a wv s =
+  let s = s.[0] <- s.[0] ^| wv.[0] ^| wv.[2] in
+  let s = s.[1] <- s.[1] ^| wv.[1] ^| wv.[3] in
+  s
+
+val blake2_compress:
+    a:alg
+  -> iv:row2 a
+  -> s:row2 a
+  -> m:block_s a
+  -> offset:limb_t a
+  -> flag:bool ->
+  Tot (row2 a)
+
+let blake2_compress a iv s m offset flag =
+  let wv = blake2_compress1 a iv s offset flag in
+  let wv = blake2_compress2 a wv m in
+  let s = blake2_compress3 a wv s in
+  s
+
+
+val blake2_update_block:
+    a:alg
+  -> iv:row2 a
+  -> flag:bool
+  -> totlen:nat{totlen <= max_limb a}
+  -> d:block_s a
+  -> s:row2 a ->
+  Tot (row2 a)
+
+let blake2_update_block a iv flag totlen d s =
+  let offset = nat_to_limb a totlen in
+  blake2_compress a iv s d offset flag
+
+val blake2_update1:
+    a:alg
+  -> iv:row2 a
+  -> prev:nat
+  -> m:bytes
+  -> i:nat{i < length m / size_block a /\ prev + length m <= max_limb a}
+  -> s:row2 a ->
+  Tot (row2 a)
+
+let get_blocki (a:alg) (m:bytes) (i:nat{i < length m / size_block a}) : block_s a =
+  Seq.slice m (i * size_block a) ((i+1) * size_block a)
+
+let blake2_update1 a iv prev m i s =
+  let totlen = prev + (i+1) * size_block a in
+  let d = get_blocki a m i in
+  blake2_update_block a iv false totlen d s
+
+val blake2_update_last:
+    a:alg
+  -> iv:row2 a
+  -> prev:nat
+  -> m:bytes{prev + length m <= max_limb a}
+  -> s:row2 a ->
+  Tot (row2 a)
+
+let get_last (a:alg) (m:bytes) : block_s a =
+  let rem = length m % size_block a in
+  let last = Seq.slice m (length m - rem) (length m) in
+  let last_block = create (size_block a) (u8 0) in
+  let last_block = update_sub last_block 0 rem last in
+  last_block
+
+let blake2_update_last a iv prev m s =
+  let totlen = prev + length m in
+  blake2_update_block a iv true totlen (get_last a m) s
+
+val blake2_update_blocks:
+    a:alg
+  -> iv:row2 a
+  -> prev:nat
+  -> m:bytes{prev + length m <= max_limb a}
+  -> s:row2 a ->
+  Tot (row2 a)
+
+let blake2_update_blocks a iv prev m s =
+  let nb = length m / size_block a in
+  let rem = length m % size_block a in
+  let nb = if rem = 0 && nb > 0 then nb - 1 else nb in
+  let rem = if rem = 0 && nb > 0 then size_block a else rem in
+  let s = repeati nb (blake2_update1 a iv prev m) s in
+  blake2_update_last a iv prev m s
+
+
+val blake2_init_hash:
+    a:alg
+  -> kk:size_nat{kk <= max_key a}
+  -> nn:size_nat{1 <= nn /\ nn <= max_output a} ->
+  Tot (row2 a & row2 a)
+
+let blake2_init_hash a kk nn =
+  let iv0 = load_row #a (map secret (sub (ivTable a) 0 4)) in
+  let iv1 = load_row #a (map secret (sub (ivTable a) 4 4)) in
+  let s0' = (nat_to_word a 0x01010000) ^. ((nat_to_word a kk) <<. (size 8)) ^. (nat_to_word a nn) in
+  let m = create_row s0' (zero a) (zero a) (zero a) in
+  let iv0' = iv0 ^| m in
+  let iv = createL [iv0;iv1] in
+  let s = createL [iv0';iv1] in
+  (iv,s)
+
+
+val blake2_init:
+    a:alg
+  -> kk:size_nat{kk <= max_key a}
+  -> k:lbytes kk
+  -> nn:size_nat{1 <= nn /\ nn <= max_output a} ->
+  Tot (row2 a & row2 a)
+
+let blake2_init a kk k nn =
+  let key_block = create (size_block a) (u8 0) in
+  let iv,s = blake2_init_hash a kk nn in
+  if kk = 0 then iv,s
+  else begin
+    let key_block = update_sub key_block 0 kk k in
+    iv,blake2_update1 a iv 0 key_block 0 s end
+
+
+val blake2_finish:
+    a:alg
+  -> s:row2 a
+  -> nn:size_nat{1 <= nn /\ nn <= max_output a} ->
+  Tot (lbytes nn)
+
+let blake2_finish a s nn =
+  let full = (uints_to_bytes_le s.[0] @| uints_to_bytes_le s.[1]) in
+  sub full 0 nn
+
+val blake2:
+    a:alg
+  -> d:bytes
+  -> kk:size_nat{kk <= max_key a /\ (if kk = 0 then length d <= max_limb a else length d + (size_block a) <= max_limb a)}
+  -> k:lbytes kk
+  -> nn:size_nat{1 <= nn /\ nn <= max_output a} ->
+  Tot (lbytes nn)
+
+let blake2 a d kk k nn =
+  let kn = if kk = 0 then 0 else 1 in
+  let prev_multi = kn * (size_block a) in
+  let iv,s = blake2_init a kk k nn in
+  let s = blake2_update_blocks a iv prev_multi d s in
+  blake2_finish a s nn
+
+val blake2s:
+    d:bytes
+  -> kk:size_nat{kk <= 32 /\ (if kk = 0 then length d < pow2 64 else length d + 64 < pow2 64)}
+  -> k:lbytes kk
+  -> nn:size_nat{1 <= nn /\ nn <= 32} ->
+  Tot (lbytes nn)
+
+let blake2s d kk k n = blake2 Blake2S d kk k n
+
+
+val blake2b:
+    d:bytes
+  -> kk:size_nat{kk <= 64 /\ (if kk = 0 then length d < pow2 128 else length d + 128 < pow2 128)}
+  -> k:lbytes kk
+  -> nn:size_nat{1 <= nn /\ nn <= 64} ->
+  Tot (lbytes nn)
+
+let blake2b d kk k n = blake2 Blake2B d kk k n
